eta-expansion yields eta-expanded terms, up to two lemmas

template-coq/theories/EtaExpand.v
@@ -56,7 +56,7 @@ Section Eta.
     let remaining_subst := mapi (subst (rev args)) remaining in 
     let remaining_combined := (combine remaining_names remaining_subst) in 
     (* let print := print_id remaining_combined in *)
-    fold_right (fun '(nm,ty) b => Ast.tLambda nm ty b) (mkApps t (prev_args ++ eta_args)) remaining_combined.
+    fold_right (fun '(nm,ty) b => Ast.tLambda nm ty b) (mkApps (lift0 needed t) (prev_args ++ eta_args)) remaining_combined.
   
   Definition eta_constructor (ind : inductive) c u args :=
       match lookup_global Σ ind.(inductive_mind) with
@@ -78,37 +78,57 @@ Section Eta.
   Definition eta_fixpoint (def : mfixpoint term) (i : nat) d (args : list term) :=
     eta_single (tFix def i) args (d.(dtype)) (1 + d.(rarg)).
 
-  Fixpoint eta_expand (t : term) : term :=
+  Definition lift_ctx n k (Γ : list (option (nat * term))) :=
+    rev (mapi (fun i x => option_map (on_snd (lift n (k + i))) x) (rev Γ)).
+
+  Definition up (Γ : list (option (nat * term))) := None :: Γ.
+
+  Fixpoint eta_expand (Γ : list (option (nat * term))) (t : term) : term :=
     match t with
+    | tVar _ | tSort _ | tProd _ _ _ | tConst _ _ | tInd _ _ => t
+    | tRel n => match nth_error Γ n with
+                | Some (Some (c, ty)) => eta_single (tRel n) [] (lift0 (S n) ty) c
+                | _ => tRel n
+                end
+  
     | tApp hd args =>
       match hd with
       | tConstruct ind c u =>
-        match eta_constructor ind c u (map eta_expand args) with 
+        match eta_constructor ind c u (map (eta_expand Γ) args) with 
         | Some res => res
         | None => tVar ("Error: lookup of an inductive failed for "
                        ++ string_of_kername ind.(inductive_mind))
         end
-      | tFix def i => let def' := (map (map_def eta_expand eta_expand) def) in 
+      | tFix def i => let def' := (map (fun d => 
+      let ctx := List.rev (mapi (fun (i : nat) d => Some (1 + d.(rarg), (lift0 i (dtype d)))) def) in
+      {| dname := dname d ; dtype := dtype d ; dbody := eta_expand (ctx ++  Γ) d.(dbody) ; rarg := rarg d |}) def) in 
                       match nth_error def' i with
-                      | Some d => eta_fixpoint def' i d (map eta_expand args)
+                      | Some d => eta_fixpoint def' i d (map (eta_expand Γ) args)
                       | None => tVar ("Error: lookup of a fixpoint failed for "
                                        ++ string_of_term t)
                       end
-      | _ => mkApps (eta_expand hd) (map eta_expand args)
+      | tRel n => match nth_error Γ n with
+                  | Some (Some (c, ty)) => eta_single (tRel n) (map (eta_expand Γ) args) (lift0 (S n) ty) c 
+                  | _ => tRel n
+                  end
+      | _ => mkApps (eta_expand Γ hd) (map (eta_expand Γ) args)
     end
-    | tEvar n ts => tEvar n (map eta_expand ts)
-    | tLambda na ty body => tLambda na ty (eta_expand body)
-    | tLetIn na val ty body => tLetIn na (eta_expand val) ty (eta_expand body)
-    | tCase p ty disc brs =>
-      tCase p ty (eta_expand disc) (map_branches eta_expand brs)
-    | tProj p t => tProj p (eta_expand t)
-    | tFix def i => let def' := (map (map_def eta_expand eta_expand) def) in 
+    | tEvar n ts => tEvar n (map (eta_expand Γ) ts)
+    | tLambda na ty body => tLambda na ty (eta_expand (up Γ) body)
+    | tLetIn na val ty body => tLetIn na (eta_expand Γ val) ty (eta_expand (up Γ) body)
+    | tCase ci p disc brs =>
+        let brs' := map (fun b => {| bcontext := bcontext b; bbody := eta_expand (repeat None #|b.(bcontext)| ++ Γ) b.(bbody) |}) brs in 
+        tCase ci p (eta_expand Γ disc) brs'
+    | tProj p t => tProj p (eta_expand Γ t)
+    | tFix def i => let def' := (map (fun d =>  
+                                         let ctx := List.rev (mapi (fun (i : nat) d => Some (1 + d.(rarg), (lift0 i (dtype d)))) def) in
+                                        {| dname := dname d ; dtype := dtype d ; dbody := eta_expand (ctx ++  Γ) d.(dbody) ; rarg := rarg d |}) def) in 
                       match nth_error def' i with
                       | Some d => eta_fixpoint def' i d []
                       | None => tVar ("Error: lookup of a fixpoint failed for "
                                        ++ string_of_term t)
                       end
-    | tCoFix def i => tCoFix (map (map_def eta_expand eta_expand) def) i
+    | tCoFix def i => tCoFix (map (map_def id (eta_expand (repeat None (#|def|) ++ Γ))) def) i
     (* NOTE: we know that constructors and constants are not applied at this point,
        since applications are captured by the previous cases *)
     | tConstruct ind c u =>
@@ -117,8 +137,7 @@ Section Eta.
         | None => tVar ("Error: lookup of an inductive failed for "
                        ++ string_of_kername ind.(inductive_mind))
         end
-    | tCast t1 k t2 => tCast (eta_expand t1) k (eta_expand t2)
-    | t => t
+    | tCast t1 k t2 => tCast (eta_expand Γ t1) k (eta_expand Γ t2)
     end.
 
 End Eta.
@@ -132,23 +151,27 @@ Fixpoint map_constants_global_declarations (f : constant_body -> constant_body) 
 
 Definition eta_global_env (Σ : global_declarations) :=
   let f cb :=
-     {| cst_type := eta_expand Σ cb.(cst_type) ; 
+     {| cst_type := eta_expand Σ [] cb.(cst_type) ; 
         cst_universes := cb.(cst_universes) ;
         cst_body := match cb.(cst_body) with
-                    | Some b => Some (eta_expand Σ b)
+                    | Some b => Some (eta_expand Σ [] b)
                     | None => None
                     end;
         cst_relevance := cb.(cst_relevance) |} in
   map_constants_global_declarations f Σ.
 
-(* 
+(*
+Inductive tree := T : list tree -> tree.
+Fixpoint tmap (f : tree -> tree) (t : tree) := match t with T l => T (map (tmap f) l) end.
 
-From MetaCoq.Template Require Import Loader.
-Variable n : nat.
-MetaCoq Quote Recursively Definition p := ltac:(let x := eval unfold Vector.append in @Vector.append in exact (x)).
-MetaCoq Unquote Definition q := (eta_expand p.1.(declarations) p.2).
+From MetaCoq.Template Require Import Loader Pretty.
+MetaCoq Quote Recursively Definition p := ltac:(let x := eval unfold tmap in tmap in exact (x)). 
+MetaCoq Unquote Definition q := (eta_expand p.1.(declarations) [] p.2). 
+Print q. 
 
-Eval cbv in let x := eta_expand p.1.(declarations) p.2 in tt.
+Eval lazy in let x := print_term (p.1, Monomorphic_ctx) [] true (eta_expand p.1.(declarations) [] p.2) in 
+             let y := print_term (p.1, Monomorphic_ctx) [] true p.2 in
+ (x,y).
 
 Print q.
 
@@ -158,6 +181,8 @@ Definition isConstruct t :=
     match t with tConstruct _ _ _ => true | _ => false end.
 Definition isFix t :=
     match t with tFix _ _ => true | _ => false end.
+Definition isRel t :=
+    match t with tRel _ => true | _ => false end.
 
 Section expanded.
 
@@ -165,116 +190,121 @@ Variable Σ : global_env.
 
 Local Unset Elimination Schemes.
 
-Inductive expanded : term -> Prop :=
-| expanded_tRel (n : nat) : expanded (tRel n)
-| expanded_tVar (id : ident) : expanded (tVar id)
-| expanded_tEvar (ev : nat) (args : list term) : Forall expanded args -> expanded (tEvar ev args)
-| expanded_tSort (s : Universe.t) : expanded (tSort s)
-| expanded_tCast (t : term) (kind : cast_kind) (v : term) : expanded t -> expanded v -> expanded (tCast t kind v)
-| expanded_tProd (na : aname) (ty : term) (body : term) : (* expanded ty -> expanded body -> *) expanded (tProd na ty body)
-| expanded_tLambda (na : aname) (ty : term) (body : term) : (* expanded ty -> *) expanded body -> expanded (tLambda na ty body)
-| expanded_tLetIn (na : aname) (def : term) (def_ty : term) (body : term) : expanded def (* -> expanded def_ty *) -> expanded body -> expanded (tLetIn na def def_ty body)
-| expanded_tApp (f : term) (args : list term) : ~ isConstruct f -> ~ isFix f -> expanded f -> Forall expanded args -> expanded (tApp f args)
-| expanded_tConst (c : kername) (u : Instance.t) : expanded (tConst c u)
-| expanded_tInd (ind : inductive) (u : Instance.t) : expanded (tInd ind u)
+Inductive expanded (Γ : list nat): term -> Prop :=
+| expanded_tRel (n : nat) : nth n Γ 0 = 0 -> expanded Γ (tRel n)
+| expanded_tRel_app (n : nat) args : nth n Γ 0 <= #|args| -> Forall (expanded Γ) args -> expanded Γ (tApp (tRel n) args)
+| expanded_tVar (id : ident) : expanded Γ (tVar id)
+| expanded_tEvar (ev : nat) (args : list term) : Forall (expanded Γ) args -> expanded Γ (tEvar ev args)
+| expanded_tSort (s : Universe.t) : expanded Γ (tSort s)
+| expanded_tCast (t : term) (kind : cast_kind) (v : term) : expanded Γ t -> expanded Γ v -> expanded Γ (tCast t kind v)
+| expanded_tProd (na : aname) (ty : term) (body : term) : (* expanded Γ ty -> expanded Γ body -> *) expanded Γ (tProd na ty body)
+| expanded_tLambda (na : aname) (ty : term) (body : term) : (* expanded Γ ty -> *) expanded (0 :: Γ) body -> expanded Γ (tLambda na ty body)
+| expanded_tLetIn (na : aname) (def : term) (def_ty : term) (body : term) : expanded Γ def (* -> expanded Γ def_ty *) -> expanded (0 :: Γ) body -> expanded Γ (tLetIn na def def_ty body)
+| expanded_tApp (f : term) (args : list term) : negb (isConstruct f || isFix f || isRel f) -> expanded Γ f -> Forall (expanded Γ) args -> expanded Γ (tApp f args)
+| expanded_tConst (c : kername) (u : Instance.t) : expanded Γ (tConst c u)
+| expanded_tInd (ind : inductive) (u : Instance.t) : expanded Γ (tInd ind u)
 | expanded_tConstruct (ind : inductive) (idx : nat) (u : Instance.t) mind idecl cdecl :
     declared_constructor Σ (ind, idx) mind idecl cdecl ->
     ind_npars mind + context_assumptions (cstr_args cdecl) = 0 ->
-    expanded (tConstruct ind idx u)
+    expanded Γ (tConstruct ind idx u)
 | expanded_tCase (ci : case_info) (type_info:predicate term)
-        (discr:term) (branches : list (branch term)) : expanded discr -> Forall (fun br => expanded br.(bbody)) branches -> expanded (tCase ci type_info discr branches)
-| expanded_tProj (proj : projection) (t : term) : expanded t -> expanded (tProj proj t)
+        (discr:term) (branches : list (branch term)) : expanded Γ discr -> Forall (fun br => expanded (repeat 0 #|br.(bcontext)| ++ Γ) br.(bbody)) branches -> expanded Γ (tCase ci type_info discr branches)
+| expanded_tProj (proj : projection) (t : term) : expanded Γ t -> expanded Γ (tProj proj t)
 | expanded_tFix (mfix : mfixpoint term) (idx : nat) args d : 
-  Forall (fun d => expanded d.(dtype) /\ expanded d.(dbody)) mfix ->
-  Forall expanded args ->
+  d.(rarg) <= #|(decompose_prod  d.(dtype)).1.1| ->
+  Forall (fun d => 
+           let ctx := List.rev (mapi (fun (i : nat) d => 1 + d.(rarg)) mfix) in
+          expanded (ctx ++ Γ) d.(dbody)) mfix ->
+  Forall (expanded Γ) args ->
   args <> [] ->
   nth_error mfix idx = Some d ->
   #|args| > d.(rarg) ->
-  expanded (tApp (tFix mfix idx) args)
+  expanded Γ (tApp (tFix mfix idx) args)
 | expanded_tCoFix (mfix : mfixpoint term) (idx : nat) : 
-  Forall (fun d => expanded d.(dtype) /\ expanded d.(dbody)) mfix ->
-  expanded (tCoFix mfix idx)
+  Forall (fun d => expanded (repeat 0 #|mfix| ++ Γ) d.(dbody)) mfix ->
+  expanded Γ (tCoFix mfix idx)
 | expanded_tConstruct_app ind c u mind idecl cdecl args :
     declared_constructor Σ (ind, c) mind idecl cdecl ->
     #|args| >= (ind_npars mind + context_assumptions (cstr_args cdecl)) ->
-    Forall expanded args ->
-    expanded (tApp (tConstruct ind c u) args).
+    Forall (expanded Γ) args ->
+    expanded Γ (tApp (tConstruct ind c u) args).
 
 End expanded.
 
 Lemma expanded_ind :
-forall (Σ : global_env) (P : term -> Prop),
-(forall n : nat, P (tRel n)) ->
-(forall id : ident, P (tVar id)) ->
-(forall (ev : nat) (args : list term), Forall (expanded Σ) args -> Forall P args -> P (tEvar ev args)) ->
-(forall s : Universe.t, P (tSort s)) ->
-(forall (t : term) (kind : cast_kind) (v : term),
- expanded Σ t -> P t -> expanded Σ v -> P v -> P (tCast t kind v)) ->
-(forall (na : aname) (ty body : term),
- (* expanded Σ ty -> P ty -> expanded Σ body -> P body -> *) P (tProd na ty body)) ->
-(forall (na : aname) (ty body : term),
- (* expanded Σ ty -> P ty -> *) expanded Σ body -> P body -> P (tLambda na ty body)) ->
-(forall (na : aname) (def def_ty body : term),
- expanded Σ def ->
- P def ->
- (* expanded Σ def_ty ->
- P def_ty -> *) expanded Σ body -> P body -> P (tLetIn na def def_ty body)) ->
-(forall (f7 : term) (args : list term),
- ~ isConstruct f7 -> ~ isFix f7 ->
- expanded Σ f7 -> P f7 -> Forall (expanded Σ) args -> Forall P args -> P (tApp f7 args)) ->
-(forall (c : kername) (u : Instance.t), P (tConst c u)) ->
-(forall (ind : inductive) (u : Instance.t), P (tInd ind u)) ->
-(forall (ind : inductive) (idx : nat) (u : Instance.t)
+forall (Σ : global_env) (P : list nat -> term -> Prop),
+(forall Γ, forall n : nat, nth n Γ 0 = 0 -> P Γ (tRel n)) ->
+(forall Γ, forall n : nat, forall args, nth n Γ 0 <= #|args| -> Forall (expanded Σ Γ) args -> Forall (P Γ) args -> P Γ (tApp (tRel n) args)) ->
+(forall Γ, forall id : ident, P Γ (tVar id)) ->
+(forall Γ, forall (ev : nat) (args : list term), Forall (expanded Σ Γ) args -> Forall (P Γ) args -> P Γ (tEvar ev args)) ->
+(forall Γ, forall s : Universe.t, P Γ (tSort s)) ->
+(forall Γ, forall (t : term) (kind : cast_kind) (v : term),
+ expanded Σ Γ t -> P Γ t -> expanded Σ Γ v -> P Γ v -> P Γ (tCast t kind v)) ->
+(forall Γ, forall (na : aname) (ty body : term), P Γ (tProd na ty body)) ->
+(forall Γ, forall (na : aname) (ty body : term), expanded Σ (0 :: Γ) body -> P (0 :: Γ) body -> P Γ (tLambda na ty body)) ->
+(forall Γ (na : aname) (def def_ty body : term),
+ expanded Σ Γ def ->
+ P Γ def ->
+ expanded Σ (0 :: Γ) body -> P (0 :: Γ) body -> P Γ (tLetIn na def def_ty body)) ->
+(forall Γ, forall (f7 : term) (args : list term),
+ negb (isConstruct f7 || isFix f7 || isRel f7) -> ~ isRel f7 ->
+ expanded Σ Γ f7 -> P Γ f7 -> Forall (expanded Σ Γ) args -> Forall (P Γ) args -> P Γ (tApp f7 args)) ->
+(forall Γ (c : kername) (u : Instance.t), P Γ (tConst c u)) ->
+(forall Γ, forall (ind : inductive) (u : Instance.t), P Γ (tInd ind u)) ->
+(forall Γ, forall (ind : inductive) (idx : nat) (u : Instance.t)
    (mind : mutual_inductive_body) (idecl : one_inductive_body)
    (cdecl : constructor_body),
  declared_constructor Σ (ind, idx) mind idecl cdecl ->
  ind_npars mind + context_assumptions (cstr_args cdecl) = 0 ->
- P (tConstruct ind idx u)) ->
-(forall (ci : case_info) (type_info : predicate term) 
+ P Γ (tConstruct ind idx u)) ->
+(forall Γ (ci : case_info) (type_info : predicate term) 
    (discr : term) (branches : list (branch term)),
- expanded Σ discr ->
- P discr ->
- Forall (fun br : branch term => expanded Σ (bbody br)) branches ->
- Forall (fun br : branch term => P (bbody br)) branches ->
- P (tCase ci type_info discr branches)) ->
-(forall (proj : projection) (t : term),
- expanded Σ t -> P t -> P (tProj proj t)) ->
-(forall (mfix : mfixpoint term) (idx : nat) d args, 
-  Forall (fun d => expanded Σ d.(dtype) /\ expanded Σ d.(dbody)) mfix -> 
-  Forall (fun d => P d.(dtype) /\ P d.(dbody)) mfix -> 
-  Forall (expanded Σ) args ->
-  Forall P args ->
+ expanded Σ Γ discr ->
+ P Γ discr ->
+ Forall (fun br : branch term => expanded Σ (repeat 0 #|br.(bcontext)| ++ Γ) (bbody br)) branches ->
+ Forall (fun br : branch term => P (repeat 0 #|br.(bcontext)| ++ Γ)%list (bbody br)) branches ->
+ P Γ (tCase ci type_info discr branches)) ->
+(forall Γ (proj : projection) (t : term),
+ expanded Σ Γ t -> P Γ t -> P Γ (tProj proj t)) ->
+(forall Γ (mfix : mfixpoint term) (idx : nat) d args, 
+  d.(rarg) <= #|(decompose_prod  d.(dtype)).1.1| ->
+  Forall (fun d =>  let ctx := List.rev (mapi (fun (i : nat) d => 1 + d.(rarg)) mfix) in expanded Σ (ctx ++ Γ) d.(dbody)) mfix -> 
+  Forall (fun d => let ctx := List.rev (mapi (fun (i : nat) d => 1 + d.(rarg)) mfix) in P (ctx ++ Γ)%list d.(dbody)) mfix -> 
+  Forall (expanded Σ Γ) args ->
+  Forall (P Γ) args ->
   args <> [] ->
   nth_error mfix idx = Some d ->
   #|args| > d.(rarg) ->
-  expanded Σ (tApp (tFix mfix idx) args) ->
-  P (tApp (tFix mfix idx) args)) ->
-(forall (mfix : mfixpoint term) (idx : nat), 
-  Forall (fun d => expanded Σ d.(dtype) /\ expanded Σ d.(dbody)) mfix -> 
-  Forall (fun d => P d.(dtype) /\ P d.(dbody)) mfix -> 
-  P (tCoFix mfix idx)) ->
-(forall (ind : inductive) (c : nat) (u : Instance.t)
+  P Γ (tApp (tFix mfix idx) args)) ->
+(forall Γ (mfix : mfixpoint term) (idx : nat), 
+  Forall (fun d => expanded Σ (repeat 0 #|mfix| ++ Γ) d.(dbody)) mfix -> 
+  Forall (fun d => P (repeat 0 #|mfix| ++ Γ)%list d.(dbody)) mfix -> 
+  P Γ (tCoFix mfix idx)) ->
+(forall Γ (ind : inductive) (c : nat) (u : Instance.t)
    (mind : mutual_inductive_body) (idecl : one_inductive_body)
    (cdecl : constructor_body) (args : list term),
  declared_constructor Σ (ind, c) mind idecl cdecl ->
  #|args| >= ind_npars mind + context_assumptions (cstr_args cdecl) ->
- Forall (expanded Σ) args ->
- Forall P args ->
- P (tApp (tConstruct ind c u) args)) -> forall t : term, expanded Σ t -> P t.
+ Forall (expanded Σ Γ) args ->
+ Forall (P Γ) args ->
+ P Γ(tApp (tConstruct ind c u) args)) -> forall Γ, forall t : term, expanded Σ Γ t -> P Γ t.
 Proof.
-  intros. revert t H16.
-  fix f 2.
-  intros t Hexp. destruct Hexp; eauto.
-  - eapply H1; eauto. induction H16; econstructor; eauto.
-  - assert (Forall P args) by (induction H18; econstructor; eauto).
-    destruct f0; eauto.
-  - eapply H11; eauto. induction H16; econstructor; eauto.
-  - eapply H13; eauto.
-    + clear - H16 f. induction H16 as [ | ? ? []]; econstructor; cbn in *; eauto; split.
-    + clear - H17 f. induction H17 as [ | ]; econstructor; cbn in *; eauto; split.
-    + eapply expanded_tFix; eauto.
-  - eapply H14; eauto. induction H16 as [ | ? ? []]; econstructor; cbn in *; eauto; split.
-  - eapply H15; eauto. clear - f H18. induction H18; econstructor; cbn in *; eauto; split.
+  intros. revert Γ t H17.
+  fix f 3.
+  intros Γ t Hexp.  destruct Hexp; eauto.
+  - eapply H0; eauto. clear - f H18. induction H18; econstructor; eauto. 
+  - eapply H2; eauto. induction H17; econstructor; eauto.
+  - assert (Forall (P Γ) args) by (induction H18; econstructor; eauto). 
+    destruct f0; cbn in *; eauto.
+  - eapply H12; eauto. induction H17; econstructor; eauto.
+  - eapply H14; eauto.
+    + clear - H18 f. revert H18.
+      generalize mfix at 1 3. intros mfix0 H18.  induction H18; econstructor; cbn in *; eauto; split.
+    + clear - H19 f. induction H19 as [ | ]; econstructor; cbn in *; eauto; split.
+  - eapply H15; eauto.
+    clear - H17 f. revert H17. 
+    generalize mfix at 1 3. intros mfix0 H17. induction H17; econstructor; cbn in *; eauto; split.
+  - eapply H16; eauto. clear - f H19. induction H19; econstructor; cbn in *; eauto; split.
 Qed.
 
 Local Hint Constructors expanded : core.
@@ -284,38 +314,31 @@ Definition isFix_app t :=
   | tFix _ _ => true
   | _ => false
   end.
+
+Definition isRel_app t :=
+  match fst (decompose_app t) with
+  | tRel _ => true
+  | _ => false
+  end.
   
-Lemma expanded_mkApps Σ f args :
-  expanded Σ f -> Forall (expanded Σ) args ->
-  ~ isConstruct_app f ->
-  ~ isFix_app f ->
-  expanded Σ (mkApps f args).
+Lemma expanded_fold_lambda Σ Γ t l :
+  expanded Σ Γ
+    (fold_right (fun '(nm, ty) (b : term) => tLambda nm ty b) t l) <->   expanded Σ (repeat 0 #|l| ++ Γ) t.
 Proof.
-  intros. destruct args; cbn.
-  - cbn. eauto.
-  - destruct f; cbn.
-    all: try now (econstructor; cbn; eauto; invs H; eauto).
-    invs H; cbn in *.
-    + econstructor; eauto. solve_all. eapply All_app_inv; eauto.
-    + exfalso. eapply H1; eauto.
-    + exfalso. eapply H1; eauto.
+  induction l as [ | []] in t, Γ |- *; cbn - [repeat] in *.
+  - reflexivity.
+  - replace (S #|l|) with (#|l| + 1) by lia.
+    rewrite repeat_app. cbn. rewrite <- app_assoc. cbn.
+    split.
+    + inversion 1; subst. now eapply IHl.
+    + intros. econstructor. now eapply IHl.
 Qed.
 
-
-Lemma expanded_fold_lambda Σ t l :
-  expanded Σ
-    (fold_right (fun '(nm, ty) (b : term) => tLambda nm ty b) t l) <->   expanded Σ t.
-Proof.
-  induction l as [ | []] in t |- *; cbn; split; firstorder.
-  eapply IHl.
-  now inversion H; subst.
-Qed.
-
-Lemma expanded_mkApps_tConstruct Σ mind idecl cdecl ind idx u args :
+Lemma expanded_mkApps_tConstruct Σ Γ mind idecl cdecl ind idx u args :
   declared_constructor Σ (ind, idx) mind idecl cdecl ->
   #|args| >= ind_npars mind + context_assumptions (cstr_args cdecl) ->
-  Forall (expanded Σ) args ->
-  expanded Σ (mkApps (tConstruct ind idx u) args).
+  Forall (expanded Σ Γ) args ->
+  expanded Σ Γ (mkApps (tConstruct ind idx u) args).
 Proof.
   intros Hdecl Heq. unfold mkApps.
   destruct args eqn:E.
@@ -323,40 +346,202 @@ Proof.
   - eapply expanded_tConstruct_app; eauto.
 Qed.
 
-Lemma expanded_mkApps_tFix Σ mfix idx d args :
+Lemma expanded_mkApps_tFix Σ Γ mfix idx d args :
+  d.(rarg) <= #|(decompose_prod  d.(dtype)).1.1| ->
   nth_error mfix idx = Some d ->
   #|args| >= S (d.(rarg)) ->
-  Forall (fun d0 : def term => expanded Σ (dtype d0) /\ expanded Σ (dbody d0)) mfix ->
-  Forall (expanded Σ) args ->
+  Forall (fun d0 : def term => let ctx := List.rev (mapi (fun (_ : nat) (d1 : def term) => 1 + rarg d1) mfix) in expanded Σ (ctx ++ Γ) (dbody d0)) mfix ->
+  Forall (expanded Σ Γ) args ->
   args <> [] ->
-  expanded Σ (mkApps (tFix mfix idx) args).
+  expanded Σ Γ (mkApps (tFix mfix idx) args).
 Proof.
   intros Hdecl Heq. unfold mkApps.
   destruct args eqn:E.
   - congruence.
   - intros. eapply expanded_tFix; eauto.
 Qed.
-
-Lemma expanded_mkApps_tFix_inv Σ mfix idx args :
-  expanded Σ (mkApps (tFix mfix idx) args) ->
-  Forall (fun d0 : def term => expanded Σ (dtype d0) /\ expanded Σ (dbody d0)) mfix.
+  
+Lemma expanded_mkApps_tFix_inv Σ Γ mfix idx args :
+  expanded Σ Γ (mkApps (tFix mfix idx) args) ->
+  Forall (fun d0 : def term => let ctx := List.rev (mapi (fun (_ : nat) (d1 : def term) => 1 + rarg d1) mfix) in expanded Σ (ctx ++ Γ) (dbody d0)) mfix.
 Proof.
   induction args.
   - cbn. inversion 1.
-  - cbn. inversion 1; subst; try congruence. now destruct H3.
+  - cbn. inversion 1; subst; cbn in *; try congruence.
 Qed.
 
-Lemma expanded_lift {Σ : global_env_ext} t n m :
-  expanded Σ t ->
-  expanded Σ (lift n m t).
+Lemma expanded_tApp_args Σ Γ t args :
+  expanded Σ Γ (tApp t args) ->
+  Forall (expanded Σ Γ) args.
 Proof.
-  induction 1 in n, m |- *; cbn; eauto.
-  all: try now (econstructor; solve_all).
-  - econstructor. destruct f7; cbn in *; congruence. destruct f7; cbn in *; congruence. eauto. solve_all.
-  - eapply expanded_tFix. solve_all. solve_all. destruct args; cbn in *; congruence. now rewrite nth_error_map, H4.
-    now rewrite map_length.
+  inversion 1; subst; eauto.
+Qed.
+
+Lemma expanded_tApps_inv Σ Γ t args :
+  expanded Σ Γ (tApp t args) ->
+  forall args', #|args'| >= #|args| ->
+  Forall (expanded Σ Γ) args' ->
+  expanded Σ Γ (tApp t args').
+Proof.
+  intros. invs H.
+  - econstructor. lia. eauto.
+  - eauto.
+  - eapply expanded_tFix; eauto.
+    destruct args, args'; cbn in *; lia || congruence.
+    lia.
   - eapply expanded_tConstruct_app; eauto.
-    now rewrite map_length. solve_all.
+    lia.
+Qed.
+
+Lemma expanded_mkApps_inv Σ Γ t args :
+  expanded Σ Γ (mkApps t args) ->
+  forall args', #|args'| >= #|args| ->
+  Forall (expanded Σ Γ) args' ->
+  expanded Σ Γ (mkApps t args').
+Proof.
+  intros.
+  destruct args' in t, args, H, H0, H1 |- *.
+  - destruct args; cbn in *; try lia. eauto.
+  - destruct args; cbn in *.
+    + destruct t; try now (eapply expanded_tApps_inv; eauto).
+      * invs H. econstructor; eauto. cbn; lia.
+      * eapply expanded_tApps_inv. eauto. len; lia.
+        eapply app_Forall; eauto. eapply expanded_tApp_args; eauto.
+      * invs H. eapply expanded_tConstruct_app; eauto. cbn; lia.
+    + destruct t; try now (eapply expanded_tApps_inv; eauto).
+      eapply expanded_tApps_inv. eauto. len; lia.
+      eapply app_Forall; eauto. eapply expanded_tApp_args in H.
+      eapply Forall_app in H. eapply H.
+Qed.
+
+Lemma expanded_mkApps Σ Γ f args :
+  expanded Σ Γ f -> Forall (expanded Σ Γ) args ->
+  expanded Σ Γ (mkApps f args).
+Proof.
+  intros. 
+  eapply expanded_mkApps_inv with (args := []); cbn; eauto. lia.
+Qed.
+
+Local Hint Rewrite repeat_length combine_length : len.
+Local Hint Rewrite <- app_assoc : list.
+
+Lemma apply_expanded Σ Γ Γ' t t' :
+  expanded Σ Γ t -> Γ = Γ' -> t = t' -> expanded Σ Γ' t'.
+Proof. intros; now subst. Qed.
+
+Lemma ext_lift n m n' m' t :
+  n' = n -> m' = m -> lift n m t = lift n' m' t.
+Proof. intros; now subst. Qed.    
+
+Lemma decompose_prod_lift t n m :
+  #|(decompose_prod t).1.1| = #|(decompose_prod (lift n m t)).1.1|.
+Proof.
+  induction t in n, m |- *; cbn; try lia.
+  destruct (decompose_prod t2) as [[]]; cbn in *.
+  specialize (IHt2 n (S m)).
+  destruct (decompose_prod (lift n (S m) t2)) as [[]]; cbn in *. lia.
+Qed.
+
+Lemma expanded_unlift {Σ : global_env} Γ' Γ'' Γ t Γgoal :
+  expanded Σ (Γ' ++ Γ'' ++ Γ) (lift #|Γ''| #|Γ'| t) ->
+  (Γ' ++ Γ)%list = Γgoal ->
+  expanded Σ Γgoal t.
+Proof.
+  intros Hexp <-.
+  remember (Γ' ++ Γ'' ++ Γ)%list as Γ_.
+  remember ((lift #|Γ''| #|Γ'| t)) as t_.
+  induction Hexp in Γ', Γ'', Γ, HeqΓ_, Heqt_, t |- *; cbn; subst; destruct t; invs Heqt_; eauto.
+  - rename n0 into n. econstructor. destruct (Nat.leb_spec #|Γ'| n).
+    + rewrite !app_nth2 in H |- *; try lia.
+      rewrite !app_nth2 in H; try lia. rewrite <- H at 2. f_equal. lia.
+    + rewrite app_nth1 in H |- *; lia.
+  - destruct t; invs H3. econstructor. 2:{ eapply Forall_map_inv in H0, H1. solve_all. }
+    revert H. len. intros H. destruct (Nat.leb_spec #|Γ'| n0).
+    + rewrite !app_nth2 in H |- *; try lia.
+      rewrite !app_nth2 in H; try lia. rewrite <- H.
+      eapply Nat.eq_le_incl. f_equal. lia.
+    + rewrite app_nth1 in H |- *; lia.    
+  - econstructor. solve_all.
+  - econstructor. rewrite app_comm_cons. eapply IHHexp; try reflexivity.
+  - econstructor; eauto. rewrite app_comm_cons. eapply IHHexp2. 2: now simpl_list. eauto.  
+  - econstructor; eauto. destruct t; cbn in *; eauto.
+    solve_all.
+  - econstructor; eauto. solve_all.
+    specialize (b (repeat 0 #|bcontext x| ++ Γ')%list Γ'' Γ).
+    autorewrite with list len in b. now  eapply b.
+  - destruct t; invs H8.
+    rewrite !nth_error_map in H5. destruct (nth_error mfix0 idx0) eqn:EE; cbn in H5; invs H5.
+    eapply expanded_tFix. 
+    + shelve.
+    + eapply Forall_map_inv in H0, H1, H3. cbn in *. 
+      solve_all. rewrite app_assoc.      
+      eapply b. autorewrite with list. f_equal. f_equal.
+      rewrite mapi_map. eapply mapi_ext. intros. cbn. reflexivity.
+      f_equal. now len.
+    + solve_all.
+    + destruct args0; cbn in *; congruence.
+    + eauto.
+    + revert H6. len. lia.
+     Unshelve. revert H6. len. cbn in *. rewrite <- decompose_prod_lift in H. lia.
+  - econstructor. solve_all. rewrite app_assoc.
+    eapply b. autorewrite with len list. reflexivity. now len.
+  - destruct t; invs H4.
+    eapply expanded_tConstruct_app; eauto. revert H0.
+    now len. solve_all.
+Qed.
+
+Lemma expanded_lift {Σ : global_env} Γ' Γ'' Γ t :
+  expanded Σ (Γ' ++ Γ) t ->
+  expanded Σ (Γ' ++ Γ'' ++ Γ) (lift #|Γ''| #|Γ'| t).
+Proof.
+  remember (Γ' ++ Γ)%list as Γ_.
+  induction 1 in Γ', Γ'', Γ, HeqΓ_ |- *; cbn; eauto; subst.
+  - econstructor. destruct (Nat.leb_spec #|Γ'| n).
+    + rewrite !app_nth2 in H |- *; try lia.
+      rewrite app_nth2; try lia. rewrite <- H. f_equal; eauto. lia.
+    + rewrite app_nth1 in H |- *; try lia.
+  - econstructor. 2: solve_all.
+    destruct (Nat.leb_spec #|Γ'| n).
+    + rewrite !app_nth2 in H |- *; try lia.
+      rewrite app_nth2; try lia. rewrite map_length, <- H.
+      eapply Nat.eq_le_incl. f_equal; eauto. lia.
+    + rewrite map_length. rewrite app_nth1 in H |- *; try lia.
+  - econstructor; solve_all.
+  - econstructor. rewrite app_comm_cons. eapply IHexpanded. now simpl_list.
+  - econstructor; eauto. rewrite app_comm_cons. eapply IHexpanded2. now simpl_list.
+  - econstructor; eauto. destruct f7; cbn in *; eauto.
+    solve_all.
+  - econstructor; eauto. solve_all.
+    specialize (a (repeat 0 #|bcontext x| ++ Γ')%list Γ'' Γ).
+    autorewrite with list len in a. now  eapply a.
+  - eapply expanded_tFix. 
+    + shelve.
+    + solve_all. eapply apply_expanded. eapply a.
+      now rewrite app_assoc. 
+      autorewrite with list. f_equal. f_equal.
+      rewrite mapi_map. eapply mapi_ext. intros. cbn. reflexivity.
+      f_equal. now len.
+    + solve_all.
+    + destruct args; cbn in *; congruence.
+    + now rewrite !nth_error_map, H5.
+    + len. lia.
+    Unshelve. cbn. rewrite H. eapply Nat.eq_le_incl.
+    now rewrite <- decompose_prod_lift.
+  - econstructor. solve_all.
+    unshelve epose proof (a (_ ++ _)%list _ _ _). 5: now rewrite <- app_assoc.
+    shelve. autorewrite with len list in H |- *. eapply H.
+  - eapply expanded_tConstruct_app; eauto.
+    now len. solve_all.
+Qed.
+
+Lemma expanded_lift' {Σ : global_env} Γ' Γ'' Γ t Γassum Γgoal n m :
+  (Γ' ++ Γ)%list = Γassum ->
+  (Γ' ++ Γ'' ++ Γ)%list = Γgoal ->
+  #|Γ''| = n -> #|Γ'| = m ->
+  expanded Σ Γassum t ->
+  expanded Σ Γgoal (lift n m t).
+Proof.
+  intros. subst. now eapply expanded_lift.
 Qed.
 
 Lemma Forall_typing_spine_Forall {cf : config.checker_flags} Σ Γ (P : term -> Prop) t_ty l t' s :
@@ -367,76 +552,394 @@ Proof.
   induction 1; econstructor; eauto.
 Qed.
 
-Lemma eta_expand_expanded {cf : config.checker_flags} {Σ : global_env_ext} Γ t T :
+Lemma nth_map' {A B} (f : A -> B) n l d d' :
+  (d' = f d) ->
+  nth n (map f l) d' = f (nth n l d).
+Proof.
+  induction n in l |- *; destruct l; simpl; auto.
+Qed.
+
+Lemma decompose_prod12 t : 
+  #| (decompose_prod t).1.1| = #|(decompose_prod t).1.2|.
+Proof.
+  induction t; cbn; try lia.
+  do 2 destruct decompose_prod as [[]]. cbn in *. lia.
+Qed.
+
+Lemma mkApps_tRel:
+forall (n : nat) (l : list term), l <> nil ->
+mkApps (tRel n) (l) = tApp (tRel n) (l).
+Proof.
+  destruct l; cbn; try congruence.
+Qed.
+
+Lemma expanded_eta_single_tRel_app Σ0 n l n0 Γ' T :
+expanded Σ0
+  (map
+     (fun x : option (nat × term) =>
+      match x with
+      | Some p => let (n1, _) := p in n1
+      | None => 0
+      end) Γ') (eta_single (tRel n) [] T n0) ->
+      Forall (expanded Σ0 
+      (map
+      (fun x : option (nat × term) =>
+       match x with
+       | Some p => let (n1, _) := p in n1
+       | None => 0
+       end) Γ')) l ->
+       n0 <= #|(decompose_prod T).1.1| ->
+expanded Σ0
+  (map
+     (fun x : option (nat × term) =>
+      match x with
+      | Some p => let (n1, _) := p in n1
+      | None => 0
+      end) Γ') (eta_single (tRel n) l T n0).
+Proof.
+  intros H Hl Hlen. unfold eta_single in *.
+  rewrite expanded_fold_lambda in H |- *.
+  rewrite Nat.sub_0_r in H. cbn in H.
+  destruct n0.
+  - cbn in *. invs H. simpl_list. eapply expanded_mkApps.
+    eauto. solve_all.
+    now rewrite lift0_id.
+  - rewrite mkApps_tRel in H. 2:
+    { replace (S n0) with (n0 + 1) by lia. rewrite rev_map_spec.
+      rewrite seq_app, map_app, rev_app_distr. cbn. congruence. }
+    invs H; cbn - [rev_map seq] in H2; try congruence.
+    autorewrite with len list in H2 |- *.
+    rewrite !firstn_length in H2 |- *.
+    rewrite !List.skipn_length. 
+    rewrite app_nth2 in H2. 2: { len. rewrite <- decompose_prod12. destruct List.length; lia. }
+    autorewrite with len in H2.
+    replace ((S (n0 + n) -
+    Init.Nat.min (Init.Nat.min (S n0) #|(decompose_prod T).1.1|)
+      (Init.Nat.min (S n0) #|(decompose_prod T).1.2|))) with n in H2. 2:{
+        rewrite <- decompose_prod12. lia.
+    }
+    unfold lift0 at 1.
+    rewrite mkApps_tRel. 2:{ destruct l; cbn - [rev_map]; try congruence. rewrite rev_map_spec. cbn. clear. destruct List.rev; cbn; try congruence. }
+    econstructor.
+    { rewrite app_length, rev_map_spec, List.rev_length, !map_length, seq_length.
+    replace ((Init.Nat.min
+    (Init.Nat.min (S n0 - #|l|) (#|(decompose_prod T).1.1| - #|l|))
+    (Init.Nat.min (S n0 - #|l|) (#|(decompose_prod T).1.2| - #|l|)))) with (S n0 - #|l|). 2:{ rewrite <- !decompose_prod12. lia. }
+    assert (0 <=? n = true) as -> by now destruct n.
+    transitivity (S n0). 2: lia.
+    rewrite app_nth2. 2:{ rewrite repeat_length; lia. }
+    rewrite repeat_length.
+    replace ((S n0 - #|l| + n - (S n0 - #|l|))) with n by lia.
+    cbn [List.length] in H2. rewrite seq_length in H2.
+    eapply H2. }
+    eapply app_Forall.
+    + Opaque minus. solve_all. eapply @expanded_lift' with (Γ' := []). cbn; reflexivity.
+      cbn; reflexivity. 2: reflexivity.
+      rewrite repeat_length, <- decompose_prod12. lia. eauto.
+    + change ((0 :: seq 1 n0)) with (seq 0 (S n0)) in *.
+      assert (S n0 > #|l| \/ S n0 <= #|l|) as [HH | HH] by lia.
+      assert (S n0 = S n0 - #|l| + #|l|) as EE by lia.
+      2:{ replace (S n0 - #|l|) with 0 by lia. cbn. econstructor. }
+      rewrite EE in H3.
+      rewrite seq_app, rev_map_spec, map_app, rev_app_distr in H3.
+      eapply Forall_app in H3 as [].
+      replace ((Init.Nat.min
+    (Init.Nat.min (S n0 - #|l|) (#|(decompose_prod T).1.1| - #|l|))
+    (Init.Nat.min (S n0 - #|l|) (#|(decompose_prod T).1.2| - #|l|)))) with (S n0 - #|l|). 2:{ rewrite <- !decompose_prod12. lia. }
+    rewrite <- EE in H0.
+    revert H0. len. rewrite !firstn_length, <- decompose_prod12.
+    replace ((Init.Nat.min (Init.Nat.min (S n0) #|(decompose_prod T).1.1|)
+    (Init.Nat.min (S n0) #|(decompose_prod T).1.1|))) with (S n0) by lia.
+    rewrite rev_map_spec. intros.
+    rewrite Forall_forall in H0 |- *. intros.
+    specialize (H0 _ H1). rewrite <- in_rev in H1.
+    eapply in_map_iff in H1 as (? & <- & [_ ?] % in_seq). 
+    invs H0.
+    econstructor. rewrite app_nth1. 2: rewrite repeat_length; lia.
+    eapply nth_repeat.
+Qed.
+
+(* Lemma expanded_eta_single_app {Σ Γ} t args args' ty count :
+  expanded Σ Γ (eta_single t args ty count) ->
+  expanded Σ Γ (eta_single t (args ++ args') ty count).
+Proof.
+  unfold eta_single. rewrite !expanded_fold_lambda.
+  rewrite !combine_length, !mapi_length, !firstn_length,  !List.skipn_length.
+  intros H.
+Admitted.  
+ *)
+
+Lemma map_repeat {A B} (f : A -> B) a n : 
+  map f (repeat a n) = repeat (f a) n.
+Proof.
+  induction n; cbn; congruence.
+Qed.
+
+
+Lemma decompose_type_of_constructor :
+  forall cf: config.checker_flags
+, forall Σ0: global_env_ext
+, forall wfΣ: wf Σ0.1
+, forall ind: inductive
+, forall i: nat
+, forall u: Instance.t
+, forall mdecl: mutual_inductive_body
+, forall idecl: one_inductive_body
+, forall cdecl: constructor_body
+, forall isdecl': declared_constructor Σ0.1 (ind, i) mdecl idecl cdecl, 
+#|(decompose_prod (type_of_constructor mdecl cdecl (ind, i) u)).1.1| = ind_npars mdecl + context_assumptions (cstr_args cdecl).
+Admitted.
+
+Lemma wf_fixpoint_rarg :
+  forall cf: config.checker_flags
+, forall Σ0: global_env_ext
+, forall wfΣ: wf Σ0.1
+, forall mfix: list (def term)
+, forall decl: def term
+, forall H2: wf_fixpoint Σ0.1 mfix, In decl mfix ->
+rarg decl < #|(decompose_prod (dtype decl)).1.2|.
+Proof. 
+Admitted.
+
+Lemma map2_length : 
+  forall {A B C : Type} (f : A -> B -> C) (l : list A) (l' : list B), #| map2 f l l'| = min #|l| #|l'|.
+Proof.
+  intros. induction l in l' |- *; cbn.
+  - reflexivity.
+  - destruct l'; cbn in *. lia. rewrite IHl. lia.
+Qed.
+
+From Equations Require Import Equations.
+
+Lemma typing_wf_fixpoint {cf : config.checker_flags} Σ0 Γ0 mfix idx t_ty  :
+   Σ0;;; Γ0 |- tFix mfix idx : t_ty -> wf_fixpoint Σ0 mfix.
+Proof.
+  intros H.
+  depind H; eauto.
+Qed.
+
+Lemma eta_expand_expanded {cf : config.checker_flags} {Σ : global_env_ext} Γ Γ' t T :
   wf Σ ->
   typing Σ Γ t T ->
-  expanded Σ (eta_expand Σ.1.(declarations) t).
+  Forall2 (fun x y => match x with Some (n, t) => y.(decl_type) = t /\ #|(decompose_prod t).1.1| >= n | None => True end) Γ' Γ ->
+  expanded Σ (map (fun x => match x with Some (n, _) => n | None => 0 end ) Γ') (eta_expand Σ.1.(declarations) Γ' t).
 Proof.
-  intros wf Hty.
-  eapply @typing_ind_env with (t := t) (Σ := Σ) (P := fun Σ Γ t T => expanded Σ (eta_expand Σ.(declarations) t)) (PΓ := fun _ _ _ => True); intros; try now (cbn; eauto).
-  - cbn. destruct (isConstruct_app t0) eqn:E.
-    + induction t0; cbn in *; try congruence.
-      unfold eta_constructor in *.
+  intros wf Hty. revert Γ'.
+  eapply @typing_ind_env with (t := t) (Σ := Σ) (P := fun Σ Γ t T => forall Γ',  Forall2 (fun (x : option (nat × term)) (y : context_decl) => match x with
+                                                               | Some (_, t0) => decl_type y = t0 /\ _
+                                                               | None => True
+                                                               end) Γ' Γ ->
+  expanded Σ (map (fun x : option (nat × term) => match x with
+                                                  | Some (n, _) => n
+                                                  | None => 0
+                                                  end) Γ') (eta_expand (declarations Σ) Γ' t)
+                                                ) (PΓ := fun _ _ _ => True); intros; try now (cbn; eauto).
+  - cbn. eapply Forall2_nth_error_Some_r in H1 as (? & ? & ?); eauto.
+    rewrite H1.
+    destruct x as [[] | ]. 
+    + destruct H2. unfold eta_single. cbn.
+      eapply expanded_fold_lambda.
+      rewrite !Nat.sub_0_r. rewrite combine_length. len.
+      destruct n0.
+      * cbn. econstructor. now rewrite nth_nth_error, nth_error_map, H1. 
+      * rewrite seq_S,rev_map_spec, map_app, rev_app_distr. cbn.
+        rewrite !firstn_length.
+         assert (#|(decompose_prod (lift0 (S n) t0)).1.1|>= S n0) by now rewrite <- decompose_prod_lift.
+         assert (#|(decompose_prod (lift0 (S n) t0)).1.2|>= S n0) by now rewrite <- decompose_prod12.
+        rewrite !Min.min_l; try lia.
+        econstructor.
+        -- rewrite app_nth2. 2: rewrite repeat_length; lia.
+           rewrite repeat_length. replace (S (n0 + n) - S n0) with n by lia.
+           rewrite nth_nth_error, nth_error_map, H1. cbn.
+           len. now rewrite seq_length.
+        -- eapply Forall_forall. intros x [ | (? & <- & [_ ?] % in_seq) % in_rev % in_map_iff]; subst.
+           all: econstructor; rewrite app_nth1; [now rewrite nth_repeat | rewrite repeat_length; lia].
+    + econstructor. now rewrite nth_nth_error, nth_error_map, H1.
+  - cbn. econstructor. eapply (H1 (up Γ')); econstructor; eauto.
+  - cbn. econstructor. eauto. eapply (H2 (up Γ')); econstructor; eauto.
+  - specialize (H _ H2).
+    assert (Forall(fun t : term => expanded Σ0 (map
+    (fun x : option (nat × term) =>
+     match x with
+     | Some p => let (n, _) := p in n
+     | None => 0
+     end) Γ') (eta_expand Σ0.(declarations) Γ' t)) l). { 
+       clear H1. clear X. induction X0; econstructor; eauto. }
+    destruct t0; cbn.
+    all: try now eapply expanded_mkApps; [ eauto | solve_all ].
+    + cbn in H.
+      destruct (nth_error Γ' n) eqn:E; eauto.
+      destruct o; eauto.
+      destruct p. cbn in *.
+      eapply expanded_eta_single_tRel_app; eauto. solve_all.
+      eapply Forall2_nth_error_Some_l in H2 as (? & ? & ?). 2: eauto. 
+      cbn in *. 
+      destruct H4.
+      rewrite <- decompose_prod_lift. lia.
+    + cbn in H. unfold eta_constructor in *.
       destruct lookup_global as [[] | ] eqn:E1; eauto.
-      destruct nth_error eqn:E2; try congruence.
-      destruct (nth_error (ind_ctors o) idx) eqn:E3; try congruence.
+      destruct nth_error eqn:E2; eauto.
+      destruct (nth_error (ind_ctors o) idx) eqn:E3; eauto. 
       unfold eta_single in H. eapply expanded_fold_lambda.
       rewrite Nat.sub_0_r in H.
       unfold mkApps in H. destruct (ind_npars m + context_assumptions (cstr_args c)) eqn:EE.
       * cbn in H. inversion H; subst. cbn.
         simpl_list. destruct l.
         -- cbn. econstructor; eauto.
-        -- cbn. eapply expanded_tConstruct_app; eauto. cbn. now rewrite H6.
-           rewrite lift0_id. erewrite map_ext. 2: eapply lift0_p. rewrite map_id.
+        -- cbn. eapply expanded_tConstruct_app; eauto. cbn. now rewrite H8.
+           rewrite lift0_id. setoid_rewrite map_ext. 3: eapply lift0_p. rewrite map_id.
            eapply Forall_typing_spine_Forall in X0.
            rewrite <- map_cons. revert X0. generalize (t0 :: l). intros l' X0.
-           solve_all.
-      * eapply expanded_mkApps_tConstruct. split. split. red. all: eauto. 
+           solve_all. eapply H4. solve_all. reflexivity.
+      * eapply expanded_mkApps_tConstruct. split. split. red. all: eauto.
         rewrite rev_map_spec. simpl_list. rewrite EE. lia. eapply Forall_typing_spine_Forall in X0.
+        assert (#|(decompose_prod (type_of_constructor m c (ind, idx) u)).1.1| = ind_npars m + context_assumptions (cstr_args c)) as E. { 
+          eapply decompose_type_of_constructor; eauto.
+          split. split. red. all: eauto. }
         eapply app_Forall.
-        -- solve_all. now eapply expanded_lift.
+        -- Opaque minus. solve_all. eapply @expanded_lift' with (Γ' := []). 2: reflexivity. reflexivity.
+           2: reflexivity. len.
+           { rewrite !firstn_length, !List.skipn_length. 
+             rewrite <- decompose_prod12, E, EE. lia.
+           }
+           cbn. eauto.
         -- rewrite rev_map_spec. eapply Forall_rev. 
-           eapply Forall_forall. intros ? (? & <- & ?) % in_map_iff. econstructor. 
-    + destruct (isFix_app t0) eqn:E2.
-      * induction t0; cbn in *; try congruence.
-        destruct (nth_error mfix idx) eqn:Eid.
-        -- rewrite (map_nth_error _ _ _ Eid) in H |- *. unfold eta_fixpoint in *.
-           eapply expanded_fold_lambda. 
-           
-           eapply expanded_mkApps_tFix.
-           ++ now rewrite nth_error_map, Eid.
-           ++ simpl_list. rewrite rev_map_spec. simpl_list. cbn. destruct #|l| eqn:?; cbn; lia.
-           ++ unfold eta_single in H.
-              rewrite expanded_fold_lambda in H.
-              eapply expanded_mkApps_tFix_inv; eauto.
-           ++ eapply Forall_typing_spine_Forall in X0. eapply app_Forall.
-              ** solve_all. now eapply expanded_lift.
-              ** rewrite rev_map_spec. eapply Forall_rev. 
-                 eapply Forall_forall. intros ? (? & <- & ?) % in_map_iff. econstructor.
-           ++ destruct l; cbn in *; try congruence. 
-        -- rewrite nth_error_map, Eid. cbn. econstructor.
-      * assert (Forall(fun t : term => expanded Σ0.1 (eta_expand Σ0.1.(declarations) t)) l). {
-        clear H1. clear X. induction X0; econstructor; eauto. }
-        induction t0; cbn.
-        all: try now (eapply expanded_mkApps; eauto; solve_all).
-        all: cbn in *; congruence.
-  - cbn. pose proof isdecl as isdecl'. destruct isdecl as [[]]. red in H1.
-    unfold lookup_env in H1.
-    unfold eta_constructor. unfold fst_ctx in *. cbn in *. rewrite H1, H2, H3.
+           eapply Forall_forall. intros ? (? & <- & ?) % in_map_iff. econstructor.
+           eapply in_seq in H4 as [_ H4].
+           len. rewrite app_nth1. 2: len.
+           eapply nth_repeat. cbn in *.
+           rewrite !firstn_length, !List.skipn_length, <- decompose_prod12, E, EE.
+           rewrite map_length in H4. lia.
+    + cbn in H. unfold eta_fixpoint in *.
+      rewrite nth_error_map in H |- *.
+      destruct (nth_error mfix idx) eqn:Eid; eauto.
+      cbn in *. 
+      eapply expanded_fold_lambda. 
+      
+      eapply expanded_mkApps_tFix; fold lift.
+      2:{rewrite !nth_error_map, Eid. reflexivity. }
+      ++ cbn. rewrite <- decompose_prod_lift. rewrite decompose_prod12.
+        eapply Nat.lt_le_incl, wf_fixpoint_rarg; eauto. 2: eapply nth_error_In; eauto.
+        clear - X. depind X; eauto.
+      ++ len. rewrite seq_length. lia.
+      ++ unfold eta_single in H.
+         rewrite expanded_fold_lambda in H. cbn. simpl_list.
+         cbn-[lift] in H. rewrite Nat.sub_0_r in H.
+         unfold lift in H. fold lift in H.
+         eapply expanded_mkApps_tFix_inv in H.
+         eapply Forall_forall.
+         intros ? (? & <- & (? & <- & ?) % in_map_iff) % in_map_iff. cbn.
+         
+         
+         eapply Forall_forall in H. 2:{ 
+         eapply in_map_iff. eexists. split. reflexivity. eapply in_map_iff. eexists. split. cbn. reflexivity. eauto. }
+         cbn in H.
+         revert H. len. intros H.
+
+         eapply typing_wf_fixpoint in X. eapply wf_fixpoint_rarg in X. 2: eauto. 2: eapply nth_error_In; eauto.
+
+         assert (#|l| > S (rarg d) \/ #|l| <= S (rarg d) )  as [He | He] by lia.
+         { replace ((S (rarg d) - #|l|)) with 0 by lia. cbn. rewrite lift0_id.
+          eapply expanded_unlift. 2: reflexivity.
+          eapply apply_expanded; eauto; len. 2:{ f_equal. instantiate (1 := repeat 0 (S (rarg d))). now len. }
+          simpl_list. rewrite !app_assoc. f_equal. f_equal.
+          2:{ f_equal. rewrite !firstn_length. rewrite decompose_prod12. lia. }
+          f_equal.  rewrite !mapi_map. now eapply mapi_ext. }
+
+         eapply expanded_unlift with (Γ'' :=  repeat 0 #|l|). 2: now rewrite <- app_assoc.
+         rewrite simpl_lift. 2:{ len. rewrite !firstn_length, !List.skipn_length. lia. }
+         2:{ len. lia. }
+         eapply apply_expanded. eauto.
+         simpl_list. f_equal. f_equal.
+         ** rewrite !mapi_map. now eapply mapi_ext.
+         ** rewrite !firstn_length, !List.skipn_length.
+            rewrite app_assoc. f_equal.
+            rewrite <- repeat_app. f_equal.
+            rewrite !decompose_prod12.           
+            lia.
+         ** f_equal. len. lia.
+      ++ eapply Forall_typing_spine_Forall in X0. eapply app_Forall.
+         ** solve_all. eapply @expanded_lift' with (Γ' := []). all: try now reflexivity. 2: eauto.
+            len. rewrite !firstn_length, !List.skipn_length.
+            eapply typing_wf_fixpoint in X.
+            eapply wf_fixpoint_rarg in X. 2: eauto. 2: eapply nth_error_In; eauto.
+            rewrite decompose_prod12. lia.
+         ** rewrite rev_map_spec. eapply Forall_rev. 
+            eapply Forall_forall. intros ? (? & <- & ?) % in_map_iff. econstructor.
+            eapply in_seq in H4 as [_ H4]. autorewrite with len in H4 |- *.
+            rewrite !firstn_length, !List.skipn_length.
+            rewrite app_nth1. eapply nth_repeat. len. 
+            eapply Nat.lt_le_trans. eauto. cbn. rewrite decompose_prod12.
+            eapply typing_wf_fixpoint in X.
+            eapply wf_fixpoint_rarg in X. 2: eauto. 2: eapply nth_error_In; eauto.
+            lia.
+      ++ destruct l; cbn in *; try congruence. 
+      ++ cbn. eauto.
+  - cbn. pose proof isdecl as isdecl'. destruct isdecl as [[]]. red in H2.
+    unfold lookup_env in H2.
+    unfold eta_constructor. unfold fst_ctx in *. cbn in *. rewrite H2, H3, H4.
     eapply expanded_fold_lambda. rewrite Nat.sub_0_r.
     eapply expanded_mkApps_tConstruct; eauto.
     rewrite rev_map_spec. now simpl_list. rewrite rev_map_spec, <- List.map_rev.
-    eapply Forall_forall. intros ? (? & <- & ?) % in_map_iff. econstructor. 
+    eapply Forall_forall. intros ? (? & <- & ?) % in_map_iff. econstructor.
+    eapply in_rev, in_seq in H5 as [_ ?]. cbn in *.
+    rewrite combine_length, mapi_length, !firstn_length. rewrite <- decompose_prod12.
+    assert (#|(decompose_prod (type_of_constructor mdecl cdecl (ind, i) u)).1.1| = ind_npars mdecl + context_assumptions (cstr_args cdecl)) as ->. {
+      eapply decompose_type_of_constructor; eauto.
+    }
+    rewrite app_nth1. now rewrite nth_repeat. rewrite repeat_length. lia.
   - cbn. econstructor; eauto. unfold map_branches. solve_all.
+    specialize (b1 (repeat None #|bcontext y| ++ Γ'))%list.
+    rewrite map_app, map_repeat in b1. eapply b1.
+    eapply Forall2_app; solve_all.
+    
+    assert (#| (case_branch_context_gen (ci_ind ci) mdecl (pparams p) 
+    (puinst p) (bcontext y) x)| = #|bcontext y|). { clear - a0.
+      unfold case_branch_context_gen. rewrite map2_length.
+      rewrite Min.min_l; try lia. eapply All2_length in a0.
+      unfold inst_case_context. unfold subst_context.
+      unfold subst_instance, subst_instance_context, map_context.
+      rewrite fold_context_k_length, map_length. unfold aname. lia.
+    }revert H9. generalize ((case_branch_context_gen (ci_ind ci) mdecl (pparams p) 
+    (puinst p) (bcontext y) x)). clear.
+    induction #|bcontext y|; intros []; cbn; intros; try congruence; econstructor; eauto.
   - cbn. rewrite nth_error_map, H0. cbn. unfold eta_fixpoint. unfold fst_ctx in *. cbn in *.
-    eapply expanded_fold_lambda. rewrite Nat.sub_0_r.
-    eapply expanded_mkApps_tFix; eauto.
-    + rewrite nth_error_map, H0. cbn. eauto.
+    eapply expanded_fold_lambda.
+    assert (#|(decompose_prod (dtype decl)).1.1| = #|(decompose_prod (dtype decl)).1.2|) as E1. { eapply decompose_prod12. }
+    assert (rarg decl < #|(decompose_prod (dtype decl)).1.2|) as E2. { eapply wf_fixpoint_rarg; eauto. now eapply nth_error_In. }
+    eapply expanded_mkApps_tFix; eauto; fold lift.
+    + rewrite <- E1 in E2. shelve.
+    + rewrite !nth_error_map, H0. cbn. eauto.
     + simpl_list. rewrite rev_map_spec. simpl_list. cbn. lia.
-    + solve_all. destruct a as (? & ? & ?). eassumption.
+    + fold lift. len. solve_all. destruct a as (? & ? & ?).
+      rewrite !firstn_length. rewrite !Nat.min_l; try lia.
+      eapply expanded_lift'.
+      5: eapply b0. 2: reflexivity. 2: now len.
+      2: now len.
+      { rewrite map_app. f_equal. rewrite map_rev. f_equal. now rewrite !mapi_map, map_mapi. }
+      eapply Forall2_app; solve_all.
+      subst types. unfold Typing.fix_context.
+      eapply All2_rev. eapply All2_mapi. eapply All_All2_refl, Forall_All, Forall_forall.
+      intros. split. reflexivity.
+      rewrite <- decompose_prod_lift.
+      eapply wf_fixpoint_rarg in H4; eauto.
+      rewrite decompose_prod12. lia.
+      Unshelve. cbn. rewrite <- decompose_prod_lift. lia.
     + cbn - [rev_map seq]. rewrite rev_map_spec. eapply Forall_rev.
       eapply Forall_forall. intros ? (? & <- & ?) % in_map_iff. econstructor.
-    + cbn - [rev_map seq]. rewrite rev_map_spec. cbn. destruct List.rev; cbn; congruence.
-  - cbn. econstructor; eauto. eapply All_Forall, All_map, All_impl. eapply (All_mix X X0). intros ? ((? & ? & ?) & ? & ?). cbn. now split.
+      eapply in_seq in H4 as [_ ?]. cbn in *.
+      rewrite combine_length, mapi_length, !firstn_length.
+      rewrite app_nth1. now rewrite nth_repeat.
+      rewrite repeat_length.
+      assert (#|(decompose_prod (dtype decl)).1.1| = #|(decompose_prod (dtype decl)).1.2|) as ->. eapply decompose_prod12.
+      lia.
+    + cbn - [rev_map seq]. rewrite rev_map_spec. cbn. rewrite Nat.sub_0_r. cbn. destruct List.rev; cbn; congruence.
+  - cbn. econstructor; eauto. eapply All_Forall, All_map, All_impl. eapply (All_mix X X0). intros ? ((? & ? & ?) & ? & ?). cbn.
+     specialize (e0 (repeat None #|mfix| ++ Γ'))%list.
+     rewrite map_app, map_repeat in e0. len. eapply e0.
+     eapply Forall2_app; eauto. unfold types.
+     assert (#|Typing.fix_context mfix| = #|mfix|). { unfold Typing.fix_context. now len. }
+     revert H4. generalize (Typing.fix_context mfix). clear.
+     induction #|mfix|; intros []; cbn; intros; try congruence; econstructor; eauto.
   - eapply typing_wf_local; eauto.
 Qed.
